ProofLibrary/AlternativeMatches/Chase.lean
@@ -1,6 +1,7 @@
 import ProofLibrary.AlternativeMatches.Basic
 import ProofLibrary.AlternativeMatches.HomomorphismExtension
 import ProofLibrary.Models.Cores
+import ProofLibrary.KnowledgeBaseBasics
 
 theorem prop_for_nat_has_minimal_such_nat (prop : Nat -> Prop) : ∀ i, prop i -> (∃ i, prop i ∧ ∀ (j : Fin i), ¬ prop j.val) := by
   intro i h
@@ -78,6 +79,107 @@ namespace GroundTermMapping
         rw [h.repeat_hom_swap] at reaches_s
         exact reaches_s
 
+  theorem repeat_each_reaches_self_of_each_reachable (h : GroundTermMapping sig) (ts : List (GroundTerm sig)) (each_reachable : ∀ t, t ∈ ts -> ∃ k, 1 ≤ k ∧ ∃ s, s ∈ ts ∧ (h.repeat_hom k) s = t) : (∀ s, s ∈ ts -> ∃ l, 1 ≤ l ∧ (h.repeat_hom l) s = s) := by
+    induction ts with
+    | nil => simp
+    | cons hd tl ih =>
+      specialize ih (by
+        intro t t_mem
+        have each_reachable_for_t := each_reachable t (by simp [t_mem])
+        rcases each_reachable_for_t with ⟨k, k_le, s, s_mem, s_eq⟩
+        simp at s_mem
+        cases s_mem with
+        | inr s_mem => exists k; constructor; exact k_le; exists s
+        | inl s_mem =>
+          have each_reachable_for_s := each_reachable s (by simp [s_mem])
+          rcases each_reachable_for_s with ⟨l, l_le, u, u_mem, u_eq⟩
+          simp at u_mem
+          cases u_mem with
+          | inl u_mem =>
+            exists (((k / l) + 1) * l)
+            constructor
+            .
+              rw [Nat.add_mul]
+              apply Nat.le_trans
+              . exact k_le
+              . apply Nat.le_of_lt
+                simp
+                -- NOTE: taken from https://github.com/leanprover-community/mathlib4/blob/3f813de52d8cffaa73e27edd62364eec90eac633/Mathlib/Data/Nat/Defs.lean#L473-L474
+                rw [← Nat.succ_mul, ← Nat.div_lt_iff_lt_mul (by apply Nat.lt_of_succ_le; exact l_le)]; exact Nat.lt_succ_self _
+            . exists t
+              constructor
+              . exact t_mem
+              . apply h.repeat_hom_move_cycle s
+                . rw [Nat.mul_comm]
+                  apply h.repeat_hom_cycle_mul
+                  rw [u_mem, ← s_mem] at u_eq
+                  exact u_eq
+                . exact s_eq
+          | inr u_mem =>
+            exists (k + l)
+            constructor
+            . apply Nat.le_add_right_of_le; exact k_le
+            . exists u
+              constructor
+              . exact u_mem
+              . rw [GroundTermMapping.repeat_hom_add]
+                rw [u_eq, s_eq]
+      )
+
+      intro s s_mem
+      simp at s_mem
+      cases s_mem with
+      | inl s_mem =>
+        specialize each_reachable s (by rw [s_mem]; simp)
+        rcases each_reachable with ⟨k, k_le, t, t_mem, t_eq⟩
+        simp at t_mem
+        cases t_mem with
+        | inl t_mem => exists k; constructor; exact k_le; rw [t_mem, ← s_mem] at t_eq; exact t_eq
+        | inr t_mem =>
+          specialize ih t t_mem
+          rcases ih with ⟨l, l_le, ih⟩
+          exists l
+          constructor
+          . exact l_le
+          . apply h.repeat_hom_move_cycle t
+            . exact ih
+            . exact t_eq
+      | inr s_mem =>
+        apply ih
+        exact s_mem
+
+  theorem repeat_globally_of_each_repeats (h : GroundTermMapping sig) (ts : List (GroundTerm sig)) (each_repeats : ∀ s, s ∈ ts -> ∃ l, 1 ≤ l ∧ (h.repeat_hom l) s = s) :
+      ∃ l, 1 ≤ l ∧ ∀ s, s ∈ ts -> (h.repeat_hom l) s = s := by
+    induction ts with
+    | nil => exists 1; simp
+    | cons hd tl ih =>
+      specialize ih (by intro s s_mem; apply each_repeats; simp [s_mem])
+      rcases ih with ⟨l_ih, l_ih_le, ih⟩
+      rcases each_repeats hd (by simp) with ⟨l_hd, l_hd_le, each_repeats⟩
+      exists l_hd * l_ih
+      constructor
+      . apply Nat.le_trans; exact l_hd_le; apply Nat.le_mul_of_pos_right; apply Nat.lt_of_succ_le; exact l_ih_le
+      . intro s s_mem
+        simp at s_mem
+        cases s_mem with
+        | inl s_mem => rw [s_mem, h.repeat_hom_cycle_mul]; exact each_repeats
+        | inr s_mem => specialize ih s s_mem; rw [Nat.mul_comm, h.repeat_hom_cycle_mul]; exact ih
+
+  theorem exists_repetition_that_is_inverse_of_closed_of_surj (h : GroundTermMapping sig) (ts : List (GroundTerm sig)) (surj : h.surjective_for_domain_and_image_list ts ts) : ∃ k, ∀ t, t ∈ ts -> (h.repeat_hom k) (h t) = t := by
+    have each_repeats := h.repeat_each_reaches_self_of_each_reachable ts (by intro t t_mem; exists 1; constructor; simp; simp [repeat_hom]; apply surj t t_mem)
+    have repeats_globally := h.repeat_globally_of_each_repeats ts each_repeats
+
+    rcases repeats_globally with ⟨k, le, repeats_globally⟩
+
+    exists k-1
+    intro t t_mem
+    have repeat_add := h.repeat_hom_add (k-1) 1 t
+    conv at repeat_add => right; right; simp [repeat_hom]
+    rw [← repeat_add]
+    rw [Nat.sub_one_add_one]
+    . apply repeats_globally; exact t_mem
+    . apply Nat.not_eq_zero_of_lt; apply Nat.lt_of_succ_le; exact le
+
 
   variable [DecidableEq sig.P]
 
@@ -125,13 +227,371 @@ namespace ChaseBranch
 
   def has_alt_match (cb : ChaseBranch obs kb) : Prop := ∃ i, cb.has_alt_match_at_step i
 
-  theorem result_isWeakCore_of_noAltMatch (cb : ChaseBranch obs kb) : ¬ cb.has_alt_match -> cb.result.isWeakCore := by
-    sorry
+  theorem result_isWeakCore_of_noAltMatch (cb : ChaseBranch obs kb) (det : kb.isDeterministic) : ¬ cb.has_alt_match -> cb.result.isWeakCore := by
+    intro noAltMatch h_0 h_0_hom
+    apply Classical.byContradiction
+    intro contra
+    have contra := implToNotOr (notAndDeMorgan contra)
 
-  theorem result_isStrongCore_of_noAltMatch (cb : ChaseBranch obs kb) : ¬ cb.has_alt_match -> cb.result.isStrongCore := by
+    have : ∀ k, (cb.branch.infinite_list k).is_none_or (fun node => ∃ (h_k : GroundTermMapping sig), (h_k.isHomomorphism cb.result cb.result) ∧ ((∀ (f : Fact sig), (∀ (t : GroundTerm sig), t ∈ f.terms -> t ∈ cb.result.terms) -> ¬ f ∈ cb.result -> h_0.applyFact f ∈ cb.result -> h_k.applyFact f ∈ cb.result) ∧ (∀ s t, s ∈ cb.result.terms -> t ∈ cb.result.terms -> s ≠ t -> h_0 s = h_0 t -> h_k s = h_k t)) ∧ (∀ t, t ∈ node.fact.val.terms -> h_k t = t)) := by
+      intro k
+      induction k with
+      | zero =>
+        rw [cb.database_first, Option.is_none_or]
+        exists h_0
+        constructor
+        . exact h_0_hom
+        . constructor
+          . constructor
+            . simp
+            . simp
+          . intro t t_mem
+            simp at t_mem
+            rcases t_mem with ⟨f, f_mem, t_mem⟩
+            cases t with
+            | inner sfs ftl =>
+              unfold Database.toFactSet at f_mem
+              simp [Set.element] at f_mem
+              unfold Fact.toFunctionFreeFact at f_mem
+              split at f_mem
+              . simp at f_mem
+              case h_2 _ _ eq =>
+                split at eq
+                case isTrue all =>
+                  rw [List.all_eq_false.mpr _] at all
+                  . simp at all
+                  . exists (FiniteTree.inner sfs ftl); constructor; exact t_mem; simp
+                . simp at eq
+            | leaf c =>
+              exact h_0_hom.left (FiniteTree.leaf c)
+      | succ k ih =>
+        cases eq : cb.branch.infinite_list (k+1) with
+        | none => simp [Option.is_none_or]
+        | some node =>
+          rw [Option.is_none_or]
+          cases eq2 : cb.branch.infinite_list k with
+          | none =>
+            have no_holes := cb.branch.no_holes (k + 1)
+            simp [eq] at no_holes
+            specialize no_holes ⟨k, by simp⟩
+            contradiction
+          | some node2 =>
+            rw [eq2, Option.is_none_or] at ih
+            rcases ih with ⟨h_k, h_k_hom, retains, identity⟩
+
+            cases eq_origin : node.origin with
+            | none =>
+              have is_some := cb.origin_is_some k
+              rw [eq, Option.is_none_or] at is_some
+              rw [eq_origin] at is_some
+              simp at is_some
+            | some origin =>
+              have node_fact_is_prev_fact_union_origin_res := cb.origin_trg_result_yields_next_node_fact k node node2 eq eq2 origin eq_origin
+              have origin_trg_active := cb.origin_trg_is_active k node node2 eq eq2
+
+              let trg_res_terms := (origin.fst.val.result.get origin.snd).terms
+
+              have h_surj_on_trg_res : h_k.surjective_for_domain_and_image_set trg_res_terms trg_res_terms := by
+                apply Classical.byContradiction
+                intro not_surj
+                apply noAltMatch
+                exists k
+                exists h_k
+                apply Or.inr
+                exists node
+                exists origin
+                constructor
+                . exact eq
+                constructor
+                . exact eq_origin
+                . constructor
+                  . constructor
+                    . exact h_k_hom.left
+                    . apply Set.subsetTransitive _ (h_k.applyFactSet cb.result) _
+                      constructor
+                      . apply GroundTermMapping.applyFactSet_subset_of_subset
+                        apply Set.subsetTransitive _ node.fact.val _
+                        constructor
+                        . rw [node_fact_is_prev_fact_union_origin_res]
+                          apply Set.subsetUnionSomethingStillSubset'
+                          apply Set.subsetOfSelf
+                        . have subset_res := chaseBranchSetIsSubsetOfResult cb (k+1)
+                          rw [eq, Option.is_none_or] at subset_res
+                          exact subset_res
+                      . exact h_k_hom.right
+                  constructor
+                  . intro t t_mem
+                    apply identity
+                    simp at t_mem
+                    rcases t_mem with ⟨v, v_mem, v_eq⟩
+                    rcases origin.fst.val.rule.frontier_var_occurs_in_fact_in_body v v_mem with ⟨a, a_mem, v_mem⟩
+                    exists origin.fst.val.subs.apply_function_free_atom a
+                    constructor
+                    . apply origin_trg_active.left
+                      rw [← List.inIffInToSet]
+                      simp [PreTrigger.mapped_body, SubsTarget.apply, GroundSubstitution.apply_function_free_conj]
+                      exists a
+                      constructor
+                      . simp [eq_origin]; exact a_mem
+                      . simp [eq_origin]
+                    . rw [← v_eq]
+                      simp [GroundSubstitution.apply_function_free_atom]
+                      exists VarOrConst.var v
+                  . unfold Function.surjective_for_domain_and_image_set at not_surj
+                    simp at not_surj
+                    rcases not_surj with ⟨t, t_mem, no_arg_for_t⟩
+                    exists t
+                    constructor
+                    . exact t_mem
+                    . intro t_mem_image
+                      rcases t_mem_image with ⟨f, f_mem, t_mem_image⟩
+                      rcases f_mem with ⟨f', f'_mem, f_eq⟩
+                      rw [← f_eq] at t_mem_image
+                      simp [GroundTermMapping.applyFact] at t_mem_image
+                      rcases t_mem_image with ⟨t', t'_mem_image, t_eq⟩
+                      apply no_arg_for_t t'
+                      . exists f'
+                      . exact t_eq
+
+              have h_surj_on_step : h_k.surjective_for_domain_and_image_set node.fact.val.terms node.fact.val.terms := by
+                rw [node_fact_is_prev_fact_union_origin_res]
+                intro t t_mem
+                rcases t_mem with ⟨f, f_mem, t_mem⟩
+                simp at f_mem
+                cases f_mem with
+                | inl f_mem =>
+                  exists t
+                  constructor
+                  . exists f; constructor; apply Or.inl; exact f_mem; exact t_mem
+                  . apply identity; exists f
+                | inr f_mem =>
+                  rcases h_surj_on_trg_res t (by exists f) with ⟨s, s_mem, s_eq⟩
+                  rcases s_mem with ⟨f', f'_mem, s_mem⟩
+                  exists s
+                  constructor
+                  . exists f'; constructor; apply Or.inr; exact f'_mem; exact s_mem
+                  . exact s_eq
+
+              have node_terms_finite := node.fact.val.terms_finite_of_finite node.fact.property
+              rcases node_terms_finite with ⟨l_terms, l_terms_nodup, l_terms_eq⟩
+
+              rw [h_k.surjective_set_list_equiv _ _ l_terms_eq _ _ l_terms_eq] at h_surj_on_step
+
+              have h_inj_on_step : h_k.injective_for_domain_list l_terms := Function.injective_of_surjective_of_nodup h_k l_terms l_terms_nodup h_surj_on_step
+              have h_closed_on_step : ∀ t, t ∈ l_terms -> h_k t ∈ l_terms := Function.closed_of_injective_of_surjective_of_nodup h_k l_terms l_terms_nodup h_inj_on_step h_surj_on_step
+
+              have inv_ex := h_k.exists_repetition_that_is_inverse_of_closed_of_surj l_terms h_surj_on_step
+              rcases inv_ex with ⟨repetition_number, inv_prop⟩
+              let inv := h_k.repeat_hom repetition_number
+
+              have extend_inv := cb.hom_for_step_extendable_result det (k+1) inv
+              rw [eq, Option.is_none_or] at extend_inv
+              specialize extend_inv (by
+                constructor
+                . apply h_k.repeat_hom_id_on_const
+                  exact h_k_hom.left
+                . have is_hom := h_k.repeat_hom_isHomomorphism cb.result h_k_hom repetition_number
+                  apply Set.subsetTransitive _ (inv.applyFactSet cb.result) _
+                  constructor
+                  . apply inv.applyFactSet_subset_of_subset
+                    have subset_res := chaseBranchSetIsSubsetOfResult cb (k+1)
+                    rw [eq, Option.is_none_or] at subset_res
+                    apply subset_res
+                  . unfold inv
+                    apply is_hom.right
+              )
+
+              rcases extend_inv with ⟨extended_inv, extended_inv_eq, extended_inv_hom⟩
+              exists extended_inv ∘ h_k
+              constructor
+              . apply GroundTermMapping.isHomomorphism_compose _ _ _ cb.result _
+                . exact h_k_hom
+                . exact extended_inv_hom
+              constructor
+              . constructor
+                . intro f terms_mem f_mem apply_mem
+                  rw [GroundTermMapping.applyFact_compose]
+                  simp
+                  apply extended_inv_hom.right
+                  apply GroundTermMapping.applyPreservesElement
+                  exact retains.left f terms_mem f_mem apply_mem
+                . intro s t s_mem t_mem neq h_0_eq
+                  simp
+                  rw [retains.right s t s_mem t_mem neq h_0_eq]
+              . intro t t_mem
+                simp
+                rw [extended_inv_eq]
+                . rw [← l_terms_eq] at t_mem
+                  unfold inv
+                  rw [inv_prop t t_mem]
+                . rw [← l_terms_eq]
+                  rw [← l_terms_eq] at t_mem
+                  apply h_closed_on_step
+                  exact t_mem
+
+    cases contra with
+    | inl not_strong =>
+      apply not_strong
+      unfold GroundTermMapping.strong
+      intro f f_dom f_mem apply_f_mem
+
+      have step_ex : ∀ (terms : List (GroundTerm sig)), (∀ t, t ∈ terms -> t ∈ cb.result.terms) -> ∃ i, (cb.branch.infinite_list i).is_some_and (fun node => ∀ t, t ∈ terms -> t ∈ node.fact.val.terms) := by
+        intro terms id_on_terms
+        induction terms with
+        | nil => exists 0; rw [cb.database_first, Option.is_some_and]; simp
+        | cons hd tl ih =>
+          rcases ih (by intro t t_mem; apply id_on_terms; simp [t_mem]) with ⟨i_ih, ih⟩
+          specialize id_on_terms hd (by simp)
+          rcases id_on_terms with ⟨f, f_mem, hd_mem⟩
+          rcases f_mem with ⟨i_hd, f_mem⟩
+
+          cases eq_hd : cb.branch.infinite_list i_hd with
+          | none => simp [eq_hd, Option.is_some_and] at f_mem
+          | some node_hd =>
+            rw [eq_hd, Option.is_some_and] at f_mem
+            cases eq_ih : cb.branch.infinite_list i_ih with
+            | none => simp [eq_ih, Option.is_some_and] at ih
+            | some node_ih =>
+              rw [eq_ih, Option.is_some_and] at ih
+              cases Decidable.em (i_hd ≤ i_ih) with
+              | inl le =>
+                exists i_ih
+                rw [eq_ih, Option.is_some_and]
+                intro t t_mem
+                simp at t_mem
+                cases t_mem with
+                | inl t_mem =>
+                  rw [t_mem]
+                  exists f
+                  constructor
+                  . have all_following := chaseBranchSetIsSubsetOfAllFollowing cb i_hd (i_ih - i_hd)
+                    simp [eq_hd] at all_following
+                    rw [Nat.add_sub_of_le le, eq_ih, Option.is_none_or] at all_following
+                    apply all_following
+                    exact f_mem
+                  . exact hd_mem
+                | inr t_mem =>
+                  apply ih
+                  exact t_mem
+              | inr lt =>
+                simp at lt
+                exists i_hd
+                rw [eq_hd, Option.is_some_and]
+                intro t t_mem
+                simp at t_mem
+                cases t_mem with
+                | inl t_mem =>
+                  rw [t_mem]
+                  exists f
+                | inr t_mem =>
+                  specialize ih t t_mem
+                  rcases ih with ⟨f', f'_mem, t_mem⟩
+                  exists f'
+                  constructor
+                  . have all_following := chaseBranchSetIsSubsetOfAllFollowing cb i_ih (i_hd - i_ih)
+                    simp [eq_ih] at all_following
+                    rw [Nat.add_sub_of_le (Nat.le_of_lt lt), eq_hd, Option.is_none_or] at all_following
+                    apply all_following
+                    exact f'_mem
+                  . exact t_mem
+
+      specialize step_ex f.terms f_dom
+      rcases step_ex with ⟨step, step_ex⟩
+
+      cases eq : cb.branch.infinite_list step with
+      | none => rw [eq, Option.is_some_and] at step_ex; contradiction
+      | some node =>
+        rw [eq, Option.is_some_and] at step_ex
+        specialize this step
+        rw [eq, Option.is_none_or] at this
+        rcases this with ⟨h_k, _, retains, identity⟩
+        have retains := retains.left f f_dom f_mem apply_f_mem
+
+        have : h_k.applyFact f = f := by
+          unfold GroundTermMapping.applyFact
+          rw [Fact.ext_iff]
+          constructor
+          . simp
+          . simp
+            apply List.map_id_of_id_on_all_mem
+            intro t t_mem
+            apply identity
+            apply step_ex
+            exact t_mem
+        apply f_mem
+        rw [← this]
+        exact retains
+    | inr not_inj =>
+      apply not_inj
+      intro s t s_mem t_mem image_eq
+      apply Classical.byContradiction
+      intro neq
+
+      rcases s_mem with ⟨f_s, f_s_mem, s_mem⟩
+      rcases t_mem with ⟨f_t, f_t_mem, t_mem⟩
+      rcases f_s_mem with ⟨step_s, f_s_mem⟩
+      rcases f_t_mem with ⟨step_t, f_t_mem⟩
+      cases eq_s : cb.branch.infinite_list step_s with
+      | none => simp [eq_s, Option.is_some_and] at f_s_mem
+      | some node_s =>
+        rw [eq_s, Option.is_some_and] at f_s_mem
+        cases eq_t : cb.branch.infinite_list step_t with
+        | none => simp [eq_t, Option.is_some_and] at f_t_mem
+        | some node_t =>
+          rw [eq_t, Option.is_some_and] at f_t_mem
+          cases Decidable.em (step_s ≤ step_t) with
+          | inl le =>
+            specialize this step_t
+            rw [eq_t, Option.is_none_or] at this
+            rcases this with ⟨h_k, _, retains, identity⟩
+            have retains := retains.right
+            specialize retains s t
+              (by exists f_s; constructor; exists step_s; rw [eq_s, Option.is_some_and]; exact f_s_mem; exact s_mem)
+              (by exists f_t; constructor; exists step_t; rw [eq_t, Option.is_some_and]; exact f_t_mem; exact t_mem)
+              neq image_eq
+            have id_s := identity s (by
+              exists f_s
+              constructor
+              . have all_following := chaseBranchSetIsSubsetOfAllFollowing cb step_s (step_t - step_s)
+                simp [eq_s] at all_following
+                rw [Nat.add_sub_of_le le, eq_t, Option.is_none_or] at all_following
+                apply all_following
+                exact f_s_mem
+              . exact s_mem
+            )
+            have id_t := identity t (by exists f_t)
+            rw [id_s, id_t] at retains
+            apply neq
+            apply retains
+          | inr lt =>
+            simp at lt
+            specialize this step_s
+            rw [eq_s, Option.is_none_or] at this
+            rcases this with ⟨h_k, _, retains, identity⟩
+            have retains := retains.right
+            specialize retains s t
+              (by exists f_s; constructor; exists step_s; rw [eq_s, Option.is_some_and]; exact f_s_mem; exact s_mem)
+              (by exists f_t; constructor; exists step_t; rw [eq_t, Option.is_some_and]; exact f_t_mem; exact t_mem)
+              neq image_eq
+            have id_s := identity s (by exists f_s)
+            have id_t := identity t (by
+              exists f_t
+              constructor
+              . have all_following := chaseBranchSetIsSubsetOfAllFollowing cb step_t (step_s - step_t)
+                simp [eq_t] at all_following
+                rw [Nat.add_sub_of_le (Nat.le_of_lt lt), eq_s, Option.is_none_or] at all_following
+                apply all_following
+                exact f_t_mem
+              . exact t_mem
+            )
+            rw [id_s, id_t] at retains
+            apply neq
+            apply retains
+
+  theorem result_isStrongCore_of_noAltMatch (cb : ChaseBranch obs kb) (det : kb.isDeterministic) : ¬ cb.has_alt_match -> cb.result.isStrongCore := by
     unfold FactSet.isStrongCore
     intro noAltMatch h endo
-    have ⟨strong, inj⟩ := cb.result_isWeakCore_of_noAltMatch noAltMatch h endo
+    have ⟨strong, inj⟩ := cb.result_isWeakCore_of_noAltMatch det noAltMatch h endo
     constructor
     . exact strong
     constructor
@@ -270,80 +730,11 @@ namespace ChaseBranch
               . rw [f_eq]; exact s_mem
 
           have : ∀ s, s ∈ prev_node.fact.val.terms -> ∃ l, 1 ≤ l ∧ (h.repeat_hom l) s = s := by
-            have aux : ∀ (l_terms : List (GroundTerm sig)), (∀ t, t ∈ l_terms -> ∀ j, ∃ k, j ≤ k ∧ ∃ s, s ∈ l_terms ∧ (h.repeat_hom k) s = t) -> (∀ s, s ∈ l_terms -> ∃ l, 1 ≤ l ∧ (h.repeat_hom l) s = s) := by
-              intro l_terms smallest
-              induction l_terms with
-              | nil => simp
-              | cons hd tl ih =>
-                specialize ih (by
-                  intro t t_mem j
-                  have smallest_for_t := smallest t (by simp [t_mem]) j
-                  rcases smallest_for_t with ⟨k, k_le, s, s_mem, s_eq⟩
-                  simp at s_mem
-                  cases s_mem with
-                  | inr s_mem => exists k; constructor; exact k_le; exists s
-                  | inl s_mem =>
-                    have smallest_for_s := smallest s (by simp [s_mem]) 1
-                    rcases smallest_for_s with ⟨l, l_le, u, u_mem, u_eq⟩
-                    simp at u_mem
-                    cases u_mem with
-                    | inl u_mem =>
-                      exists (((k / l) + 1) * l)
-                      constructor
-                      .
-                        rw [Nat.add_mul]
-                        apply Nat.le_trans
-                        . exact k_le
-                        . apply Nat.le_of_lt
-                          simp
-                          -- NOTE: taken from https://github.com/leanprover-community/mathlib4/blob/3f813de52d8cffaa73e27edd62364eec90eac633/Mathlib/Data/Nat/Defs.lean#L473-L474
-                          rw [← Nat.succ_mul, ← Nat.div_lt_iff_lt_mul (by apply Nat.lt_of_succ_le; exact l_le)]; exact Nat.lt_succ_self _
-                      . exists t
-                        constructor
-                        . exact t_mem
-                        . apply h.repeat_hom_move_cycle s
-                          . rw [Nat.mul_comm]
-                            apply h.repeat_hom_cycle_mul
-                            rw [u_mem, ← s_mem] at u_eq
-                            exact u_eq
-                          . exact s_eq
-                    | inr u_mem =>
-                      exists (k + l)
-                      constructor
-                      . apply Nat.le_add_right_of_le; exact k_le
-                      . exists u
-                        constructor
-                        . exact u_mem
-                        . rw [GroundTermMapping.repeat_hom_add]
-                          rw [u_eq, s_eq]
-                )
-
-                intro s s_mem
-                simp at s_mem
-                cases s_mem with
-                | inl s_mem =>
-                  specialize smallest s (by rw [s_mem]; simp) 1
-                  rcases smallest with ⟨k, k_le, t, t_mem, t_eq⟩
-                  simp at t_mem
-                  cases t_mem with
-                  | inl t_mem => exists k; constructor; exact k_le; rw [t_mem, ← s_mem] at t_eq; exact t_eq
-                  | inr t_mem =>
-                    specialize ih t t_mem
-                    rcases ih with ⟨l, l_le, ih⟩
-                    exists l
-                    constructor
-                    . exact l_le
-                    . apply h.repeat_hom_move_cycle t
-                      . exact ih
-                      . exact t_eq
-                | inr s_mem =>
-                  apply ih
-                  exact s_mem
             intro s s_mem
             rw [l_terms_eq] at s_mem
-            apply aux l_terms
-            . intro t t_mem j
-              specialize smallest t (by rw [l_terms_eq]; exact t_mem) j
+            apply h.repeat_each_reaches_self_of_each_reachable l_terms
+            . intro t t_mem
+              specialize smallest t (by rw [l_terms_eq]; exact t_mem) 1
               rcases smallest with ⟨k, k_le, u, u_mem, u_eq⟩
               rw [l_terms_eq] at u_mem
               exists k
@@ -352,26 +743,9 @@ namespace ChaseBranch
               . exists u
             . exact s_mem
 
-
           -- swapped quantifiers in previous this
           have : ∃ l, 1 ≤ l ∧ ∀ s, s ∈ prev_node.fact.val.terms -> (h.repeat_hom l) s = s := by
-            have aux : ∀ (l_terms : List (GroundTerm sig)), (∀ s, s ∈ l_terms -> ∃ l, 1 ≤ l ∧ (h.repeat_hom l) s = s) -> ∃ l, 1 ≤ l ∧ ∀ s, s ∈ l_terms -> (h.repeat_hom l) s = s := by
-              intro l_terms precond
-              induction l_terms with
-              | nil => exists 1; simp
-              | cons hd tl ih =>
-                specialize ih (by intro s s_mem; apply precond; simp [s_mem])
-                rcases ih with ⟨l_ih, l_ih_le, ih⟩
-                rcases precond hd (by simp) with ⟨l_hd, l_hd_le, precond⟩
-                exists l_hd * l_ih
-                constructor
-                . apply Nat.le_trans; exact l_hd_le; apply Nat.le_mul_of_pos_right; apply Nat.lt_of_succ_le; exact l_ih_le
-                . intro s s_mem
-                  simp at s_mem
-                  cases s_mem with
-                  | inl s_mem => rw [s_mem, h.repeat_hom_cycle_mul]; exact precond
-                  | inr s_mem => specialize ih s s_mem; rw [Nat.mul_comm, h.repeat_hom_cycle_mul]; exact ih
-            rcases aux l_terms (by intro s s_mem; rw [← l_terms_eq] at s_mem; apply this; exact s_mem) with ⟨l, l_le, aux⟩
+            rcases h.repeat_globally_of_each_repeats l_terms (by intro s s_mem; rw [← l_terms_eq] at s_mem; apply this; exact s_mem) with ⟨l, l_le, aux⟩
             exists l
             constructor
             . exact l_le
